move composition to distributed system level, needed for invariants

working/composition/event_based_refinement/load_balancer/compositional/abstract_composition/ComposedDistributedSystem.t.dfy
@@ -1,60 +1,137 @@
 include "../shared/Types.t.dfy"
-include "../shared/Host.t.dfy"
-include "ComposedSpec.t.dfy"
 include "ComposedNetwork.t.dfy"
 
 // analogous to module AbstractDistributedSystem
 abstract module ComposedDistributedSystem {
     import opened Types
-    import Network: ComposedNetwork
+    import opened Network: ComposedNetwork
 
     datatype Constants = Constants(
-        hosts: seq<Network.Host.Constants>,
+        dsA: Spec.DSA.Constants,
+        dsB: Spec.DSB.Constants,
         network: Network.Constants) 
     {
         ghost predicate WF() 
         {
-            && Network.Host.GroupWFConstants(hosts)
+            && dsA.WF()
+            && dsB.WF()
         }
     }
 
     datatype Variables = Variables(
-        hosts: seq<Network.Host.Variables>,
+        dsA: Spec.DSA.Variables,
+        dsB: Spec.DSB.Variables,
         network: Network.Variables) 
     {
         ghost predicate WF(c: Constants) {
             && c.WF()
-            && |c.hosts| == |hosts|
-            && Network.Host.GroupWFVariables(c.hosts, hosts)
+            && dsA.WF(c.dsA)
+            && dsB.WF(c.dsB)
         }
     }
 
     ghost predicate Init(c: Constants, v: Variables) {
         && v.WF(c)
-        && (forall i :: 0 <= i < |c.hosts| ==> Network.Host.Init(c.hosts[i], v.hosts[i]))
+        && Spec.DSA.Init(c.dsA, v.dsA)
+        && Spec.DSB.Init(c.dsB, v.dsB)
         && Network.Init(c.network, v.network)
     }
 
-    ghost predicate HostAction(c: Constants, v: Variables, v': Variables, evt: Option<Network.Host.Spec.Event>, hostId: nat, msgOps: Network.Host.MessageOps)
+    ghost predicate IsEventA(evt: Option<Spec.Event>) 
+    {
+        || evt.None?
+        || (evt.Some? && evt.value.EventA?)
+    }
+
+    ghost function UnwrapEventA(evt: Option<Spec.Event>) : Option<Spec.DSA.Network.Host.Spec.Event>
+        requires IsEventA(evt)
+    {
+        if evt.Some? then Some(evt.value.evtA) else None
+    }
+
+    ghost predicate IsEventB(evt: Option<Spec.Event>)
+    {
+        || evt.None?
+        || (evt.Some? && evt.value.EventB?)
+    }
+
+    ghost function UnwrapEventB(evt: Option<Spec.Event>) : Option<Spec.DSB.Network.Host.Spec.Event>
+        requires IsEventB(evt)
+    {
+        if evt.Some? then Some(evt.value.evtB) else None
+    }
+
+     ghost predicate IsMessageOpsA(msgOps: ComposedMessageOps) 
+    {
+        && (|| msgOps.recv.None?
+            || (msgOps.recv.Some? && msgOps.recv.value.MessageA?))
+        && (|| msgOps.send.None?
+            || (msgOps.send.Some? && msgOps.send.value.MessageA?))
+    }
+
+    ghost function UnwrapMessageOpsA(msgOps: ComposedMessageOps): Spec.DSA.Network.Host.MessageOps
+        requires IsMessageOpsA(msgOps)
+    {
+        Spec.DSA.Network.Host.MessageOps(
+            if msgOps.recv.None? then None else Some(msgOps.recv.value.msgA),
+            if msgOps.send.None? then None else Some(msgOps.send.value.msgA)
+        )
+    }
+
+    ghost predicate IsMessageOpsB(msgOps: ComposedMessageOps)
+    {
+        && (|| msgOps.recv.None?
+            || (msgOps.recv.Some? && msgOps.recv.value.MessageB?))
+        && (|| msgOps.send.None?
+            || (msgOps.send.Some? && msgOps.send.value.MessageB?))
+    }
+
+    ghost function UnwrapMessageOpsB(msgOps: ComposedMessageOps): Spec.DSB.Network.Host.MessageOps
+        requires IsMessageOpsB(msgOps)
+    {
+        Spec.DSB.Network.Host.MessageOps(
+            if msgOps.recv.None? then None else Some(msgOps.recv.value.msgB),
+            if msgOps.send.None? then None else Some(msgOps.send.value.msgB)
+        )
+    }
+
+    ghost predicate DSAAction(c: Constants, v: Variables, v': Variables, evt: Option<Spec.Event>, msgOps: ComposedMessageOps)
+        requires v.WF(c)
+        requires v'.WF(c)
+    {
+        && IsEventA(evt)
+        && IsMessageOpsA(msgOps)
+        && (exists hostId :: Spec.DSA.NextStep(c.dsA, v.dsA, v'.dsA, UnwrapEventA(evt), Spec.DSA.HostActionStep(hostId, UnwrapMessageOpsA(msgOps))))
+        && v.dsB == v'.dsB
+    }
+
+    ghost predicate DSBAction(c: Constants, v: Variables, v': Variables, evt: Option<Spec.Event>, msgOps: ComposedMessageOps)
+        requires v.WF(c)
+        requires v'.WF(c)
+    {
+        && IsEventB(evt)
+        && IsMessageOpsB(msgOps)
+        && (exists hostId :: Spec.DSB.NextStep(c.dsB, v.dsB, v'.dsB, UnwrapEventB(evt), Spec.DSB.HostActionStep(hostId, UnwrapMessageOpsB(msgOps))))
+        && v.dsB == v'.dsB
+    }
+
+    ghost predicate DSAction(c: Constants, v: Variables, v': Variables, evt: Option<Spec.Event>, msgOps: ComposedMessageOps)
     {
         && v.WF(c)
         && v'.WF(c)
-        && 0 <= hostId < |v.hosts|
-        && Network.Host.Next(c.hosts[hostId], v.hosts[hostId], v'.hosts[hostId], evt, msgOps)
-        && (forall i :: 0 <= i < |v.hosts| && i != hostId ==> v.hosts[i] == v'.hosts[i])
-        && (forall i :: 0 <= i < |v.hosts| ==> v.hosts[i] == v'.hosts[i])        
+        && (DSAAction(c, v, v', evt, msgOps) || DSBAction(c, v, v', evt, msgOps))
         && Network.Next(c.network, v.network, v'.network, msgOps)
     }
 
     datatype Step =
-        | HostActionStep(hostId: nat, msgOps: Network.Host.MessageOps)
+        | DSActionStep(msgOps: ComposedMessageOps)
 
-    ghost predicate NextStep(c: Constants, v: Variables, v': Variables, evt: Option<Network.Host.Spec.Event>, step: Step)
+    ghost predicate NextStep(c: Constants, v: Variables, v': Variables, evt: Option<Spec.Event>, step: Step)
     {
-        && HostAction(c, v, v', evt, step.hostId, step.msgOps)
+        && DSAction(c, v, v', evt,step.msgOps)
     }
 
-    ghost predicate Next(c: Constants, v: Variables, v': Variables, evt: Option<Network.Host.Spec.Event>)
+    ghost predicate Next(c: Constants, v: Variables, v': Variables, evt: Option<Spec.Event>)
     //{
     //    exists step :: NextStep(c, v, v', evt, step)
     //}
