working/composition/event_based_refinement/load_balancer/compositional/abstract_composition/ComposedNetwork.t.dfy
@@ -1,21 +1,35 @@
 include "../shared/Types.t.dfy"
-include "ComposedHost.t.dfy"
+include "ComposedSpec.t.dfy"
+include "../shared/DistributedSystem.t.dfy"
 
 // analogous to module AbstractNetwork
 abstract module ComposedNetwork {
     import opened Types
-    import opened Host : ComposedHost
+    import opened Spec: ComposedSpec
+
+    datatype ComposedMessage = MessageA(msgA: DSA.Network.Host.Message) | MessageB(msgB: DSB.Network.Host.Message)
+    datatype ComposedMessageOps = MessageOps(recv:Option<ComposedMessage>, send:Option<ComposedMessage>, send_trans:Option<ComposedMessage>)
+
+    ghost predicate TranslateAToB(msgA: DSA.Network.Host.Message, msgB: DSB.Network.Host.Message)
+    ghost predicate TranslateBToA(msgB: DSB.Network.Host.Message, msgA: DSA.Network.Host.Message)
+
+    ghost predicate Translate(fromMsg: Option<ComposedMessage>, toMsg: Option<ComposedMessage>) {
+        match (fromMsg, toMsg)
+        case (Some(MessageA(_)), Some(MessageB(_))) => TranslateAToB(fromMsg.value.msgA, toMsg.value.msgB)
+        case (Some(MessageB(_)), Some(MessageA(_))) => TranslateBToA(fromMsg.value.msgB, toMsg.value.msgA)
+        case _ => false
+    }
 
     datatype Constants = Constants
 
-    datatype Variables = Variables(sentMsgs:set<Message>)
+    datatype Variables = Variables(sentMsgs:set<ComposedMessage>)
 
     ghost predicate Init(c: Constants, v: Variables)
     {
         && v.sentMsgs == {}
     }
 
-    ghost predicate Next(c: Constants, v: Variables, v': Variables, msgOps: MessageOps)
+    ghost predicate Next(c: Constants, v: Variables, v': Variables, msgOps: ComposedMessageOps)
     {
         && (msgOps.recv.Some? ==> msgOps.recv.value in v.sentMsgs)
         && v'.sentMsgs == v.sentMsgs
