working/composition/event_based_refinement/load_balancer/compositional/abstract_composition/ComposedSpec.t.dfy
@@ -1,23 +1,23 @@
 include "../shared/Spec.t.dfy"
-include "../shared/Host.t.dfy"
+include "../shared/DistributedSystem.t.dfy"
 
 abstract module ComposedSpec refines AbstractSpec {
-    import HostA : AbstractHost
-    import HostB : AbstractHost
+    import DSA : AbstractDistributedSystem
+    import DSB : AbstractDistributedSystem
 
-    datatype Event = EventA(evtA: HostA.Spec.Event) | EventB(evtB: HostB.Spec.Event)
+    datatype Event = EventA(evtA: DSA.Network.Host.Spec.Event) | EventB(evtB: DSB.Network.Host.Spec.Event)
 
-    datatype Constants = Constants(cnstsA: HostA.Spec.Constants, cnstsB: HostB.Spec.Constants)
-    datatype Variables = Variables(varsA: HostA.Spec.Variables, varsB: HostB.Spec.Variables)
+    datatype Constants = Constants(cnstsA: DSA.Network.Host.Spec.Constants, cnstsB: DSB.Network.Host.Spec.Constants)
+    datatype Variables = Variables(varsA: DSA.Network.Host.Spec.Variables, varsB: DSB.Network.Host.Spec.Variables)
 
     ghost predicate Init(c: Constants, v: Variables) {
-        && HostA.Spec.Init(c.cnstsA, v.varsA)
-        && HostB.Spec.Init(c.cnstsB, v.varsB)
+        && DSA.Network.Host.Spec.Init(c.cnstsA, v.varsA)
+        && DSB.Network.Host.Spec.Init(c.cnstsB, v.varsB)
     }
 
     ghost predicate Next(c: Constants, v: Variables, v': Variables, evt: Event) {
         match evt 
-        case EventA(_) => HostA.Spec.Next(c.cnstsA, v.varsA, v'.varsA, evt.evtA) && v.varsB == v'.varsB
-        case EventB(_) => HostB.Spec.Next(c.cnstsB, v.varsB, v'.varsB, evt.evtB) && v.varsA == v'.varsA
+        case EventA(_) => DSA.Network.Host.Spec.Next(c.cnstsA, v.varsA, v'.varsA, evt.evtA) && v.varsB == v'.varsB
+        case EventB(_) => DSB.Network.Host.Spec.Next(c.cnstsB, v.varsB, v'.varsB, evt.evtB) && v.varsA == v'.varsA
     }
 }
