working/composition/event_based_refinement/load_balancer/compositional/client_server/ClientServerNetwork.t.dfy
@@ -1,6 +1,20 @@
 include "../abstract_composition/ComposedNetwork.t.dfy"
-include "ClientServerHost.v.dfy"
+include "ClientServerSpec.t.dfy"
 
 module ClientServerNetwork refines ComposedNetwork {
-    import opened Host = ClientServerHost
+    import opened Spec = ClientServerSpec
+
+    ghost predicate TranslateAToB(msgA: DSA.Network.Host.Message, msgB: DSB.Network.Host.Message)
+    {
+        && msgA.ClientRequest?
+        && msgB.ServerRequest?
+        && msgA.request == msgB.request
+    }
+
+    ghost predicate TranslateBToA(msgB: DSB.Network.Host.Message, msgA: DSA.Network.Host.Message)
+    {
+        && msgB.ServerResponse?
+        && msgA.ClientResponse?
+        && msgB.response == msgA.response
+    }
 }
