working/composition/event_based_refinement/load_balancer/compositional/client_server/ClientServerDistributedSystem.t.dfy
@@ -2,5 +2,5 @@ include "../abstract_composition/ComposedDistributedSystem.t.dfy"
 include "ClientServerNetwork.t.dfy"
 
 module ClientServerDistributedSystem refines ComposedDistributedSystem {
-    import Network = ClientServerNetwork
+    import opened Network = ClientServerNetwork
 }
