working/composition/event_based_refinement/load_balancer/compositional/server/DistributedSystem.v.dfy
@@ -1,6 +1,6 @@
 include "../shared/DistributedSystem.t.dfy"
 include "Network.v.dfy"
 
-module DistributedSystem refines AbstractDistributedSystem {
+module ServerDistributedSystem refines AbstractDistributedSystem {
     import Network = ServerNetwork
 }
